theories/Prover.v
@@ -1,12 +1,8 @@
-Require Import Coq.Bool.Bool.
-Require Import ExtLib.Structures.EqDep.
-Require Import ExtLib.Tactics.Consider.
-Require Import ExtLib.Data.HList.
-Require Import MirrorCore.Iso.
+Require Import Coq.Lists.List Coq.Bool.Bool.
+Require Import ExtLib.Tactics.
 Require Import MirrorCore.TypesI.
 Require Import MirrorCore.ExprI.
 Require Import MirrorCore.EnvI.
-Require Import MirrorCore.ExprProp.
 
 Set Implicit Arguments.
 Set Strict Implicit.
@@ -18,14 +14,15 @@ Section proverI.
   Context {RType_typ : RType typD}.
   Variable expr : Type.
   Context {Expr_expr : Expr typD expr}.
-  Context {typ0_prop : TypInstance0 typD Prop}.
+  Context {ty : typ}.
+  Variable Provable' : typD nil ty -> Prop.
 
-  (** TODO:
-   ** It may be adventageous to have a non-prop prover, to allow
-   ** asking to prove equality facts.
-   ** Additionally, restricting ourselves to goals denoted by
-   ** [expr] implies that you are limited by what you can express.
-   **)
+  Let Provable (us vs : env typD) (e : expr) : Prop :=
+    match exprD us vs e ty with
+      | None => False
+      | Some val => Provable' val
+    end.
+
 
   Record Prover : Type :=
   { Facts : Type
@@ -43,24 +40,39 @@ Section proverI.
       valid uvars vars sum ->
       forall goal,
         prover sum (typeof_env uvars) (typeof_env vars) goal = true ->
-        Safe_expr (typeof_env uvars) (typeof_env vars) goal (@typ0 _ _ _ typ0_prop) ->
-        Provable typ0_prop uvars vars goal.
-
+        match exprD uvars vars goal ty with
+          | None => True
+          | Some val => Provable' val
+        end.
 
   Record ProverOk (P : Prover) : Type :=
   { Valid : env typD -> env typD -> Facts P -> Prop
   ; Valid_weaken : forall u g f ue ge,
     Valid u g f -> Valid (u ++ ue) (g ++ ge) f
   ; Summarize_correct : forall (uvars vars : env typD) (hyps : list expr),
-    Forall (Provable (expr := expr) typ0_prop uvars vars) hyps ->
+    Forall (Provable uvars vars) hyps ->
     Valid uvars vars (Summarize P (typeof_env uvars) (typeof_env vars) hyps)
   ; Learn_correct : forall uvars vars facts,
     Valid uvars vars facts -> forall hyps,
-    Forall (Provable typ0_prop uvars vars) hyps ->
+    Forall (Provable uvars vars) hyps ->
     Valid uvars vars (P.(Learn) facts (typeof_env uvars) (typeof_env vars) hyps)
   ; Prove_correct : ProveOk Valid P.(Prove)
   }.
 
+  Theorem Prove_concl P (Pok : ProverOk P)
+  : forall (vars uvars : env typD)
+           (sum : Facts P),
+      Valid Pok uvars vars sum ->
+      forall (goal : expr),
+        Prove P sum (typeof_env uvars) (typeof_env vars) goal = true ->
+        forall val,
+          exprD uvars vars goal ty = Some val ->
+          Provable' val.
+  Proof.
+    intros.
+    specialize (@Pok.(Prove_correct) vars uvars sum H goal H0).
+    rewrite H1. exact (fun x => x).
+  Qed.
 
   (** Composite Prover **)
   Section composite.
@@ -93,9 +105,8 @@ Section proverI.
        try destruct facts; intuition eauto).
       unfold ProveOk. destruct sum; intuition.
       consider (Prove pl f (typeof_env uvars) (typeof_env vars) goal); intros.
-      eapply Prove_correct0; eassumption.
-      eapply Prove_correct1; eassumption.
+      { eapply Prove_correct0; eassumption. }
+      { eapply Prove_correct1; eassumption. }
     Qed.
   End composite.
 End proverI.
-
